Lean/Egg/Core/Encode/EncodeM.lean
@@ -1,6 +1,5 @@
 import Egg.Core.Config
 import Egg.Core.Source
-import Egg.Core.Encode.IndexT
 import Std.Data.List.Basic
 
 open Lean
@@ -9,17 +8,17 @@ namespace Egg
 
 structure EncodeM.State where
   exprSrc : Source
-  config  : Config
+  config  : Config.Encoding
   bvars   : List FVarId := []
 
-abbrev EncodeM := StateT EncodeM.State <| IndexT MetaM
+abbrev EncodeM := StateT EncodeM.State MetaM
 
 namespace EncodeM
 
 def exprSrc : EncodeM Source :=
   State.exprSrc <$> get
 
-def config : EncodeM Egg.Config:=
+def config : EncodeM Config.Encoding :=
   State.config <$> get
 
 -- Note: This only works as intended if `m` does not add any additional bvars (permanently).
@@ -33,14 +32,6 @@ def withInstantiatedBVar (ty body : Expr) (m : Expr → EncodeM α) : EncodeM α
 
 def bvarIdx? (id : FVarId) : EncodeM (Option Nat) := do
   return (← get).bvars.indexOf? id
-
--- Note: If `m` changes the value of `typeTags` it will not be preserved.
-def withTypeTags (typeTags : Config.TypeTags) (m : EncodeM α) : EncodeM α := do
-  let s ← get
-  set { s with config.typeTags := typeTags }
-  let a ← m
-  set { s with config.typeTags := s.config.typeTags }
-  return a
 
 -- TODO: Only erasing proofs if they don't contain mvars, i.e. if `!e.hasMVar` can cause problems.
 --       E.g. if we have a goal equality where the lhs contains a proof term, it will probably
