Lean/Egg/Core/Encode/Basic.lean
@@ -7,10 +7,13 @@ namespace Egg
 
 abbrev Expression := String
 
+private def Expression.erased : Expression :=
+  "_"
+
 -- Note: The encoding of expression mvars and universe level mvars in rewrites relies on the fact
 --       that their indices are also unique between eachother.
 
-def encodeLevel : Level → Source → Expression
+private def encodeLevel : Level → Source → Expression
   | .zero,       _     => "0"
   | .succ l,     k     => s!"(succ {encodeLevel l k})"
   | .max l₁ l₂,  k     => s!"(max {encodeLevel l₁ k} {encodeLevel l₂ k})"
@@ -19,35 +22,24 @@ def encodeLevel : Level → Source → Expression
   | .mvar id,    _     => s!"?{id.uniqueIdx!}"
   | .param name, _     => s!"(param {name})"
 
-open EncodeM IndexT
+open EncodeM
 
 -- Note: This function expects its input expression to be normalized (cf. `Egg.normalize`).
-partial def encode (e : Expr) (src : Source) (cfg : Config) : IndexT MetaM Expression :=
-  Prod.fst <$> (go e).run { exprSrc := src, config := cfg }
+partial def encode (e : Expr) (src : Source) (cfg : Config) : MetaM Expression :=
+  Prod.fst <$> (go e).run { exprSrc := src, config := cfg.toEncoding }
 where
   go (e : Expr) : EncodeM Expression := do
-    if ← needsProofErasure e then return "proof" else
-      let c ← core e
-      if (← config).typeTags == .none || e.isSort || e.isForall then return c else
-        let some tag ← getTypeTag? e | unreachable!
-        return s!"(τ {tag} {c})"
-
-  getTypeTag? (e : Expr) : EncodeM (Option Expression) := do
-    let ty ← Meta.inferType e
-    match (← config).typeTags with
-    | .indices => return s!"{← typeIdx ty}"
-    | .exprs   => withTypeTags .none do core ty
-    | .none    => return none
+    if ← needsProofErasure e then return Expression.erased else core e
 
   core : Expr → EncodeM Expression
     | .bvar idx         => return s!"(bvar {idx})"
     | .fvar id          => encodeFVar id
     | .mvar id          => encodeMVar id
     | .sort lvl         => return s!"(sort {encodeLevel lvl (← exprSrc)})"
-    | .const name lvls  => return s!"(const {name}{← encodeULvls lvls})"
+    | .const name lvls  => return s!"(const {name}{← encodeConstLvls lvls})"
     | .app fn arg       => return s!"(app {← go fn} {← go arg})"
-    | .lam _ ty b _     => withInstantiatedBVar ty b (return s!"(λ {← go ·})")
-    | .forallE _ ty b _ => withInstantiatedBVar ty b (return s!"(∀ {← go ·})")
+    | .lam _ ty b _     => encodeLam ty b
+    | .forallE _ ty b _ => encodeForall ty b
     | .lit (.strVal l)  => return s!"(lit \"{l}\")"
     | .lit (.natVal l)  => return s!"(lit {l})"
     | _                 => panic! "'Egg.encode.core' received non-normalized expression"
@@ -62,7 +54,17 @@ where
     | .goal => return s!"(mvar {id.uniqueIdx!})"
     | _     => return s!"?{id.uniqueIdx!}"
 
-  encodeULvls (lvls : List Level) : EncodeM Expression := do
-    if (← config).eraseULvls
-    then return ""
+  encodeConstLvls (lvls : List Level) : EncodeM Expression := do
+    if (← config).eraseConstLevels
+    then return s!" {Expression.erased}"
     else return lvls.foldl (init := "") (s!"{·} {encodeLevel · (← exprSrc)}")
+
+  encodeLam (ty b : Expr) : EncodeM Expression :=
+    withInstantiatedBVar ty b fun body => do
+      let dom ← if (← config).eraseLamdaDomains then return Expression.erased else go ty
+      return s!"(λ {dom} {← go body})"
+
+  encodeForall (ty b : Expr) : EncodeM Expression :=
+    withInstantiatedBVar ty b fun body => do
+      let dom ← if (← config).eraseForallDomains then return Expression.erased else go ty
+      return s!"(∀ {dom} {← go body})"
