Lean/Egg/Tactic/Basic.lean
@@ -1,8 +1,8 @@
 import Egg.Core.Request
+import Egg.Core.Explanation.Proof
 import Egg.Core.TcProjs
 import Egg.Tactic.Config
-import Egg.Tactic.Explanation.Parse
-import Egg.Tactic.Explanation.Proof
+import Egg.Tactic.Explanation
 import Egg.Tactic.Base
 import Egg.Tactic.Rewrites
 import Egg.Tactic.Trace
@@ -27,13 +27,11 @@ private structure M.State where
   rws  : Rewrites
   dirs : Array Rewrite.Directions
 
-private abbrev M := ReaderT M.State <| IndexT <| TacticM
+private abbrev M := ReaderT M.State TacticM
 
-private def parseGoal (goal : MVarId) (reduce : Bool) (base? : Option (TSyntax `egg_base)) :
+private def parseGoal (goal : MVarId) (base? : Option (TSyntax `egg_base)) :
     MetaM M.State.Goal := do
-  let mut goalType ← goal.getType'
-  if reduce then goalType ← reduceAll goalType
-  goalType ← normalize goalType
+  let goalType ← normalize (← goal.getType')
   let base? ← base?.mapM parseBase
   let cgr ← getCongr goalType base?
   return { id := goal, type := cgr, base? }
@@ -48,7 +46,7 @@ where
 
 private def genRewrites (goal : M.State.Goal) (rws : TSyntax `egg_rws) (cfg : Config) :
     TacticM Rewrites := do
-  let mut rws ← Rewrites.parse cfg.reduce rws
+  let mut rws ← Rewrites.parse rws
   unless cfg.genTcProjRws do return rws
   let targets := #[(goal.type, Source.goal)] ++ (rws.map fun rw => (rw.toCongr, rw.src))
   return rws ++ (← genTcProjReductions targets)
@@ -79,12 +77,6 @@ private def traceFrontend : M Unit := do
           trace[egg.frontend] "Directions: {dir}"
       if cfg.genNatLitRws then
         trace[egg.frontend] "Nat Literal Conversions"
-    if cfg.typeTags == .indices then
-      withTraceNode `egg.frontend (fun _ => return "Types") do
-        let types ← IndexT.getTypes
-        for idx in [:types.size], ty in types do
-          withTraceNode `egg.frontend (fun _ => return m!"{idx}") (collapsed := false) do
-            trace[egg.frontend] ty
 
 private def processRawExpl (rawExpl : Explanation.Raw) : M Unit := do
   if rawExpl.isEmpty then throwError "egg failed to prove goal"
@@ -95,30 +87,33 @@ private def processRawExpl (rawExpl : Explanation.Raw) : M Unit := do
     goal.id.admit
   else
     let expl ← rawExpl.parse
-    let mut proof ← expl.proof goal.type (← rws) cfg
+    let mut proof ← expl.proof goal.type (← rws)
     -- When `goal.base? = some base`, then `proof` is a proof of `base = <goal type>`. We turn this
     -- into a proof of `<goal type>` here.
     if let some base := goal.base? then proof ← mkEqMP proof (.fvar base)
     goal.id.assign proof
 
 def mkRequest : M Request := do
-  Request.from (← goal).type (← rws) (← dirs) (← cfg)
+  Request.encoding (← goal).type (← rws) (← dirs) (← cfg)
 
-def runWithFreshIndex (s : M.State) (m : M α) : TacticM α :=
-  IndexT.withFreshIndex (m.run s)
+def run (s : M.State) (m : M α) : TacticM α :=
+  m.run s
 
 end M
 
 open M
 
+-- TODO: When constructing the `dirs`, there is a mismatch between `ignoreULvls` and
+--       `eraseConstLevels` when it comes to `Expr.sort`. This might cause egg to crash due to
+--       unbound mvars.
 elab "egg " cfg:egg_cfg rws:egg_rws base:(egg_base)? : tactic => do
   let goal ← getMainGoal
   let cfg ← Config.parse cfg
   goal.withContext do
-    let goal ← parseGoal goal cfg.reduce base
+    let goal ← parseGoal goal base
     let rws ← genRewrites goal rws cfg
-    let dirs ← rws.validDirs! cfg.eraseULvls
-    runWithFreshIndex { goal, cfg, rws, dirs } do
+    let dirs ← rws.validDirs! (ignoreULvls := cfg.eraseConstLevels)
+    run { goal, cfg, rws, dirs } do
       let request ← mkRequest
       traceFrontend
       if cfg.exitPoint == .beforeEqSat then goal.id.admit; return
