Lean/Egg/Tactic/Explanation.lean
@@ -1,4 +1,4 @@
-import Egg.Core.Explanation
+import Egg.Core.Explanation.Basic
 
 open Lean
 
@@ -7,6 +7,7 @@ namespace Egg.Explanation
 declare_syntax_cat egg_expl
 declare_syntax_cat egg_expl_step
 declare_syntax_cat egg_lvl
+declare_syntax_cat egg_lvls
 declare_syntax_cat egg_lit
 declare_syntax_cat egg_rw_dir
 declare_syntax_cat egg_side
@@ -22,6 +23,9 @@ syntax "(" &"param" ident ")"          : egg_lvl
 syntax "(" &"succ" egg_lvl ")"         : egg_lvl
 syntax "(" &"max" egg_lvl egg_lvl ")"  : egg_lvl
 syntax "(" &"imax" egg_lvl egg_lvl ")" : egg_lvl
+
+syntax egg_lvl* : egg_lvls
+syntax "_"      : egg_lvls
 
 syntax num : egg_lit
 syntax str : egg_lit
@@ -52,20 +56,17 @@ syntax egg_fwd_rw_src (noWs "-rev")? : egg_rw_src
 --       functions below. For example, expression type tags should never contain a "Rewrite", but we
 --       just ignore this.
 
+syntax "_"                                                         : egg_expl_step
 syntax "(" &"bvar" num ")"                                         : egg_expl_step
 syntax "(" &"fvar" num ")"                                         : egg_expl_step
 syntax "(" &"mvar" num ")"                                         : egg_expl_step
 syntax "(" &"sort" egg_lvl ")"                                     : egg_expl_step
-syntax "(" &"const" ident egg_lvl* ")"                             : egg_expl_step
+syntax "(" &"const" ident egg_lvls ")"                             : egg_expl_step
 syntax "(" &"app" egg_expl_step egg_expl_step ")"                  : egg_expl_step
-syntax "(" &"λ" egg_expl_step ")"                                  : egg_expl_step
-syntax "(" &"∀" egg_expl_step ")"                                  : egg_expl_step
+syntax "(" &"λ" egg_expl_step egg_expl_step ")"                    : egg_expl_step
+syntax "(" &"∀" egg_expl_step egg_expl_step ")"                    : egg_expl_step
 syntax "(" &"lit" egg_lit ")"                                      : egg_expl_step
 syntax "(" &"Rewrite" noWs egg_rw_dir egg_rw_src egg_expl_step ")" : egg_expl_step
--- TODO: A more efficient way of handling type tags would be to declare a separate category for them
---       where one case is `num` and the other is an expression of the form `(.*)` such that parens
---       are balanced.
-syntax "(" &"τ" (num <|> egg_expl_step) egg_expl_step ")"          : egg_expl_step
 
 syntax egg_expl_step+ : egg_expl
 
@@ -77,6 +78,11 @@ private partial def parseLevel : (TSyntax `egg_lvl) → Level
   | `(egg_lvl|(max $lvl₁ $lvl₂))  => .max (parseLevel lvl₁) (parseLevel lvl₂)
   | `(egg_lvl|(imax $lvl₁ $lvl₂)) => .imax (parseLevel lvl₁) (parseLevel lvl₂)
   | _                             => unreachable!
+
+private def parseLevels : (TSyntax `egg_lvls) → Option (Array Level)
+  | `(egg_lvls|$[$lvls]*) => lvls.map parseLevel
+  | `(egg_lvls|_)         => none
+  | _                     => unreachable!
 
 private def parseLit : (TSyntax `egg_lit) → Literal
   | `(egg_lit|$n:num) => .natVal n.getNat
@@ -144,17 +150,17 @@ private partial def parseExplStep (stx : TSyntax `egg_expl_step) : ParseStepResu
   return (← e, info?)
 where
   go (pos : SubExpr.Pos) : (TSyntax `egg_expl_step) → ParseStepM Expression
+    | `(egg_expl_step|_)                        => return .erased
     | `(egg_expl_step|(bvar $idx))              => return .bvar idx.getNat
     | `(egg_expl_step|(fvar $id))               => return .fvar (.fromUniqueIdx id.getNat)
     | `(egg_expl_step|(mvar $id))               => return .mvar (.fromUniqueIdx id.getNat)
     | `(egg_expl_step|(sort $lvl))              => return .sort (parseLevel lvl)
-    | `(egg_expl_step|(const $name $lvls*))     => return .const name.getId (lvls.map parseLevel)
+    | `(egg_expl_step|(const $name $lvls))      => return .const name.getId (parseLevels lvls)
     | `(egg_expl_step|(app $fn $arg))           => return .app (← go pos.pushAppFn fn) (← go pos.pushAppArg arg)
-    | `(egg_expl_step|(λ $body))                => return .lam (← go pos.pushBindingBody body)
-    | `(egg_expl_step|(∀ $body))                => return .forall (← go pos.pushBindingBody body)
+    | `(egg_expl_step|(λ $ty $body))            => return .lam (← go pos.pushBindingDomain ty) (← go pos.pushBindingBody body)
+    | `(egg_expl_step|(∀ $ty $body))            => return .forall (← go pos.pushBindingDomain ty) (← go pos.pushBindingBody body)
     | `(egg_expl_step|(lit $l))                 => return .lit (parseLit l)
     | `(egg_expl_step|(Rewrite$dir $src $body)) => parseRw dir src body pos
-    | `(egg_expl_step|(τ $_ $e))                => go pos e
     | _                                         => unreachable!
 
   parseRw (dir : TSyntax `egg_rw_dir) (src : TSyntax `egg_rw_src) (body : TSyntax `egg_expl_step)
