Lean/Egg/Tests/EraseConstLvls.lean
@@ -1,0 +1,11 @@
+import Egg
+
+-- Tests for manually inspecting what terms look like with or without constant level erasure.
+set_option trace.egg true
+
+-- TODO: https://leanprover.zulipchat.com/#narrow/stream/270676-lean4/topic/Unify.20level.20mvars
+example : 0 = 0 := by
+  egg (config := { eraseConstLevels := true })
+
+example : 0 = 0 := by
+  egg (config := { eraseConstLevels := false })
