Lean/Egg/Tests/Soundness.lean
@@ -1,15 +1,10 @@
 import Egg
 
--- Tests containing examples of (potential) soundness issues.
+-- Tests containing examples of backend soundness issues.
 
 -- Note: The `sorry` indicates that egg found a proof, but we're not performing proof reconstruction
 --       (which would be impossible) as a result of setting `exitPoint := .beforeProof`.
 example : False := by
   have h : ∀ x : Unit, x = .unit := fun _ => rfl
-  have : 1 + 2 = 0 := by egg (config := { typeTags := .none, exitPoint := .beforeProof }) [h]
+  have : 1 + 2 = 0 := by egg (config := { exitPoint := .beforeProof }) [h]
   contradiction
-
-example : True := by
-  have h : ∀ x : Unit, x = .unit := fun _ => rfl
-  fail_if_success have : 1 + 2 = 0 := by egg (config := { typeTags := .indices }) [h]
-  constructor
